Jan8-9

b.v
@@ -35,6 +35,16 @@ Definition is_honest (n:node):Prop
     := is_honest_bool n = true.
 
 
+Definition node_eq_dec := Nat.eq_dec.
+
+Lemma set_mem_iff_list_in: 
+    forall n:node, forall setx: set node,
+    set_mem node_eq_dec n setx = true <-> In n setx.
+    intros.
+    split.
+    - apply set_mem_correct1.
+    - apply set_mem_correct2.
+Qed.
 
 Hypothesis committee_size: forall s:slot, forall n:node, 
     length (local_committees n s) = n_committee.
@@ -42,15 +52,26 @@ Hypothesis committee_size: forall s:slot, forall n:node,
 Hypothesis committee_in_nodes: forall s:slot, forall n:node, 
     incl (local_committees n s) nodes.
 
+Lemma com_in_nodes: forall s:slot, forall n_v: node, 
+    forall n_com:node,
+    set_mem node_eq_dec n_com (local_committees n_v s) = true -> set_mem node_eq_dec n_com nodes = true.
+    intros.
+    apply set_mem_iff_list_in in H.
+    rewrite set_mem_iff_list_in.
+    apply committee_in_nodes with (s:=s)(n:=n_v). auto.
+Qed.
+
 Definition is_committee_maj_honest (nodes: set node): Prop:=
     let honest_nodes:= filter is_honest_bool nodes in
     2*(length honest_nodes) > length nodes.
 
 
-Definition node_eq_dec := Nat.eq_dec.
 
-Definition in_committee_for (n:node) (s:slot) (view: node): bool:=
+Definition in_committee_for_bool (n:node) (s:slot) (view: node): bool:=
     set_mem node_eq_dec n (local_committees view s).
+
+Definition in_committee_for (n:node) (s:slot) (view: node): Prop:=
+    set_mem node_eq_dec n (local_committees view s) = true.
 
 Definition is_honest_node (n:node):Prop:=
     is_honest n /\ set_mem node_eq_dec n nodes = true.
@@ -59,6 +80,7 @@ Definition is_honest_node_bool (n:node):bool:=
 
 Variable delta: nat. (* the communication delay *)
 Variable interact_duration: nat. (* the time for proposal-voting-aggregation step *)
+Variable slot_duration: nat. (* the upper limit of time from entering slot to confirming a block *)
 
 Record PlainProposalType: Type := mkPlainProposal {
     pr_slot: slot;
@@ -127,6 +149,7 @@ Record CertProofType: Type := mkCertProof {
 }.
 
 Inductive MsgContentType: Type :=
+    | aggProposalMsg (aggProposal: AggregatedProposalType)
     | leaderProposalMsg (leaderProposal:LeaderProposalType)
     | ackMsg (ack: AckType)
     | quitMsg (qt: QuitType).
@@ -151,6 +174,8 @@ Definition fullblock2hash (block: FullBlockType): nat:=
     aggblock2hash block.(bk_proposal).(lp_ap).
 Definition fullblock_prevhash (block: FullBlockType): nat:=
     block.(bk_proposal).(lp_ap).(ap_proposal).(pr_prevhash).
+Definition fullblock2aggblock (block: FullBlockType): AggregatedProposalType:=
+    block.(bk_proposal).(lp_ap).
 
 Variable agg_prevblock: AggregatedProposalType->FullBlockType. 
 Definition full_prevblock (block: FullBlockType): FullBlockType:=
@@ -174,7 +199,7 @@ Definition is_fullblock_valid (block: FullBlockType): Prop:=
     True. (* left as TODO *)
 
 Definition block_equal (b1 b2: FullBlockType): Prop:=
-    True. (* left as TODO *) 
+    fullblock2aggblock b1 = fullblock2aggblock b2. (* left as TODO *) 
 
 (* ##### Part 2 ends *)
 
@@ -230,8 +255,6 @@ Fixpoint state_after_node_id (n:node) (i:nat): State:=
 
 Variable confirmed_blocks: node->slot->option FullBlockType. 
 
-Variable confirm_time: node->slot->nat. (* should also be option type? no. Valid only if confirmed_blocks n s is not None *)
- 
 Variable enter_slot_seqid: node->slot->nat. 
 Definition enter_slot_time (n:node) (s:slot):=
     match node_id_to_event n (enter_slot_seqid n s) with 
@@ -245,14 +268,76 @@ Definition confirm_slot_time (n:node) (s:slot):=
     | Some ev => ev.(ev_time)
     end. 
 
+Variable honest_winner_block: slot->AggregatedProposalType.
+
+Variable certified_blocks: node->slot->nat->option LeaderProposalType. (* round *)
+
+Variable acknowledged_blocks: node->slot->nat->option LeaderProposalType.
+
 (* ##### Part 4 ends *)
 
 (* ##### Part 5: Triggers | many assumptions are here *)
 
 (* assumption - honest committee members receive the largest honest winner block on time. *)
 
+Lemma nonemptyset_exists: 
+    forall setx: set node,
+    length setx > 0 -> exists n:node, set_mem node_eq_dec n setx = true.
+    intros.
+    destruct_with_eqn setx.
+    inversion H.
+    exists n. simpl. unfold node_eq_dec.
+    destruct (Nat.eq_dec n n); auto. 
+Qed.
+
+
+
+Lemma setfilter_cond:
+    forall setx: set node, forall f: node->bool,
+    let subset:= filter f setx in
+    forall n:node, set_mem node_eq_dec n subset = true -> set_mem node_eq_dec n setx = true /\ f n = true.
+    intros.
+    apply set_mem_iff_list_in in H.
+    rewrite set_mem_iff_list_in.
+    apply filter_In.
+    auto.
+Qed.
+
+
 Hypothesis honest_majority: forall s:slot, forall n:node, 
     is_honest_node n -> is_committee_maj_honest (local_committees n s).
+
+Hypothesis exists_honest_node:
+    exists h_n:node, is_honest_node h_n.
+
+
+Lemma exists_honest_com_node:
+    forall s:slot, forall n_v:node,
+    is_honest_node n_v ->
+    exists n_hc:node,  in_committee_for n_hc s n_v /\ is_honest_node n_hc.
+    intros.
+    pose proof H as G.
+    apply honest_majority with (s:=s)(n:=n_v) in G .
+    unfold is_committee_maj_honest in G.
+    remember (local_committees n_v s) as coms.
+    remember (filter is_honest_bool coms) as honest_coms.
+    assert (length honest_coms >0).
+    lia.
+    assert (exists n:node, set_mem node_eq_dec n honest_coms = true).
+    apply nonemptyset_exists. auto.
+    destruct H1.
+    exists x. 
+    unfold in_committee_for.
+    rewrite <- Heqcoms. 
+
+    (* a node from honest_coms is both honest and in_com *)
+    rewrite Heqhonest_coms in H1.
+    unfold is_honest_node.
+    apply setfilter_cond in H1.
+    destruct H1. split. auto. split. auto.
+    
+    apply com_in_nodes with (s:=s)(n_v:=n_v). rewrite <- Heqcoms. auto.
+Qed.
 
 Hypothesis confirmed_block_none_keeps_none: forall s:slot, forall n:node, 
     confirmed_blocks n s = None -> confirmed_blocks n (S s) = None.
@@ -270,21 +355,44 @@ Hypothesis confirm_slot_sync: (* enter slot is defined as 1 unit of time after c
         confirm_slot_time n1 s <= (confirm_slot_time n2 s) + delta. 
 (* Don't need enter slot time anymore. *)
 
-Hypothesis receive 
+
+
+Hypothesis receive_honest_winner_block:
+    forall s:slot, forall n:node, forall b: FullBlockType, 
+    is_honest_node n ->
+    confirmed_blocks n s = Some b ->
+    exists i:nat, exists ev: Event,
+    node_id_to_event n i = Some ev /\
+    ev.(ev_trigger) = trigger_msg (aggProposalMsg (honest_winner_block (s+1))) /\ (ev.(ev_time) > ((confirm_slot_time n s) + delta)) /\ (ev.(ev_time) < ((confirm_slot_time n s) + interact_duration)).
+
 
 (* ##### Part 5 ends *)
 
 (* ##### Part 6: Intermediate Lemmas *)
-
-
-Lemma once_commit_all_commit:
-    forall s:slot, forall n1 n2:node, forall block: FullBlockType, 
+Lemma one_commit_other_committed:
+    forall s:slot, forall n1 n2:node, forall block1: FullBlockType, 
     is_honest_node n1 -> is_honest_node n2 ->
-    confirmed_blocks n1 s = Some block ->
-    confirmed_blocks n2 s = Some block /\ confirm_time n2 s <= confirm_time n1 s + delta. 
-Admitted. (* todo, how to define confirm. How does the communication work. *)
+    confirmed_blocks n1 s = Some block1 ->
+    exists block2: FullBlockType,
+    confirmed_blocks n2 s = Some block2.
+Admitted. 
+
+Definition confirm_same_block_pred (s:slot): Prop:=
+    exists aggProposal: AggregatedProposalType, forall n:node,
+    is_honest_node n ->
+    exists block: FullBlockType,
+    confirmed_blocks n s = Some block /\ fullblock2aggblock block = aggProposal.
 
 (* here not mentioning the time *)
+
+
+Lemma commit_implies_honest_certify:
+    forall s:slot, forall n:node, forall fb:FullBlockType,
+    is_honest_node n ->
+    confirmed_blocks n s = Some fb ->
+    exists com:node, is_honest_node com /\ in_committee_for com s n /\ let lp:= fb.(bk_proposal) in
+    certified_blocks com s lp.(lp_round) = Some lp.
+Admitted. 
 
 (* ##### Part 6 ends *)
 
@@ -293,62 +401,188 @@ Admitted. (* todo, how to define confirm. How does the communication work. *)
 
 (* ##### Part 7: Big Lemmas *)
 
+
 Hypothesis committee_determined_by_prevblocks:
     forall s:slot, forall n1 n2:node, forall block1 block2: FullBlockType,
     is_honest_node n1 -> is_honest_node n2 ->
     confirmed_blocks n1 s = Some block1 -> 
     confirmed_blocks n2 s = Some block2 ->
     block_equal block1 block2 ->
+    local_committees n1 (S s) = local_committees n2 (S s).
+
+Hypothesis committee_same_s0:
+    forall n1 n2:node, 
+    is_honest_node n1 -> is_honest_node n2 ->
+    local_committees n1 0 = local_committees n2 0.
+
+Variable lp_in_ackproof_node_slot_round: LeaderProposalType->node->slot->nat->Prop.
+
+
+Lemma block_implies_committee_same_s1:
+    forall s:slot, 
+    confirm_same_block_pred s ->
+    exists coms: set node, forall n:node, is_honest_node n ->
+    local_committees n (S s) = coms. 
+
+    intros.
+    (* strategy choice: assume that there exist an honest node. use its coms.  *)
+    destruct exists_honest_node as [n_h].
+    remember (local_committees n_h (S s)) as coms.
+    exists coms.
+    intros.
+    unfold confirm_same_block_pred in H.
+    destruct H as [aggProposal].
+
+    pose proof H0 as H0'.
+    apply H in H0'.
+    destruct H0' as [block1].
+    destruct H2.
+
+    pose proof H1 as H1'.
+    apply H in H1'.
+    destruct H1' as [block2].
+    destruct H4.
+
+    assert (block_equal block2 block1).
+    unfold block_equal. rewrite H3. rewrite H5. auto.
+    
+    rewrite Heqcoms.
+    apply committee_determined_by_prevblocks with (s:=s)(n1:=n)(n2:=n_h) (block1:=block2)(block2:=block1). auto. auto. auto. auto. auto. 
+Qed.
+
+
+Lemma block_implies_committee_pair_equal_s1:
+    forall s:slot, 
+    confirm_same_block_pred s ->
+    forall n1 n2:node,
+    is_honest_node n1 -> is_honest_node n2 ->
     local_committees n1 s = local_committees n2 s.
 
-Lemma safety_slot_induction_s0:
-    forall n1 n2: node, forall block1 block2: FullBlockType,
-    is_honest_node n1 -> is_honest_node n2 ->
-    confirmed_blocks n1 0 = Some block1 ->
-    confirmed_blocks n2 0 = Some block2 ->
-    block_equal block1 block2.
 Admitted.
 
-Lemma safety_slot_induction_s1: (* actually requiring that everyone reaches consensus on the block of *)
-    forall s:slot, forall n1 n2: node, forall block1 block2: FullBlockType, forall block1' block2': FullBlockType,
-    is_honest_node n1 -> is_honest_node n2 ->
-    confirmed_blocks n1 s = Some block1 -> 
-    confirmed_blocks n2 s = Some block2 ->
-    block_equal block1 block2 -> (* the above is the condition that previous block are the same. *)
-    in_committee_for n1 (S s) n1 = true -> 
-    in_committee_for n2 (S s) n2 = true -> 
-    confirmed_blocks n1 (S s) = Some block1' -> 
-    confirmed_blocks n2 (S s) = Some block2' ->
-    block_equal block1' block2'.
+(* same slot, same round implication. *)
+Lemma honest_cert_implies_honest_ack:
+    forall s:slot, 
+    (s = 0 \/ confirm_same_block_pred (s-1)) ->
+    forall r:nat, forall lp:LeaderProposalType,
+    forall n:node, is_honest_node n ->
+    in_committee_for n s n ->
+    certified_blocks n s r = Some lp ->
+    (exists n':node, is_honest_node n' -> in_committee_for n' s n' -> acknowledged_blocks n' s r = Some lp).
+
 Admitted. 
 
-Lemma liveness_slot_induction_s0:
-    forall n:node, 
-    is_honest_node n -> 
-    exists i: nat, 
-    let state_i:= state_after_node_id n i in
-    state_i.(st_slot) = 0 /\
-    (exists block: FullBlockType,
-    state_i.(st_committed_block) = Some block).
+(* assuming honest majority implicitly *)
+Lemma important_lemma: 
+    forall s:slot, 
+    (s = 0 \/ confirm_same_block_pred (s-1)) ->
+    forall n:node, forall lp: LeaderProposalType,
+    is_honest_node n ->
+    certified_blocks n s lp.(lp_round) = Some lp ->
+    (forall n': node, is_honest_node n' -> (* saved the ack-witness in round lp_round *)
+    in_committee_for n' s n' ->
+    lp_in_ackproof_node_slot_round lp n' s lp.(lp_round)) /\ (* part 1: every other has ackproof *)
+    (forall n'':node, is_honest_node n''->
+    in_committee_for n'' s n'' ->
+    exists lp':LeaderProposalType, acknowledged_blocks n'' s lp.(lp_round) = Some lp'-> lp' = lp).
 Admitted.
 
-Lemma liveness_slot_induction_s1:
-    forall s:slot, forall n:node, forall i:nat, 
-    is_honest_node n ->(
-    let state_i:= state_after_node_id n i in
-    state_i.(st_slot) = s /\
+Lemma comH_ackproofed_implies_no_conflict_honest_ack:
+    forall s:slot, 
+    (s = 0 \/ confirm_same_block_pred (s-1)) ->
+    forall r:nat, forall lp:LeaderProposalType,
+    (forall n:node, is_honest_node n ->
+    in_committee_for n s n ->
+    lp_in_ackproof_node_slot_round lp n s r) ->
+    (forall r':nat, forall n':node, forall lp':LeaderProposalType, is_honest_node n' -> r<=r'  -> acknowledged_blocks n' s r' = Some lp'-> lp'.(lp_ap) = lp.(lp_ap)).
+Admitted.
+
+(* proof-chain: enter slot sync -> receive honest winner sync -> ! not required in safety, only required in liveness. *)
+
+(* as long as every committee member of slot s, enters slot s with at most delta delay among each other, confirming on the same block in slot s-1 -> every node, will confirm the same block in slot s. With delta delay. *)
+Lemma safety_per_slot_helper:
+    forall s:slot, 
+    (s = 0 \/ confirm_same_block_pred (s-1)) ->
+    forall n1 n2:node, forall block1 block2: FullBlockType,
+    is_honest_node n1 -> is_honest_node n2 ->
+    confirmed_blocks n1 s = Some block1 ->
+    confirmed_blocks n2 s = Some block2 ->
+    let lp1:= block1.(bk_proposal) in
+    let lp2:= block2.(bk_proposal) in
+    lp1.(lp_round) <= lp2.(lp_round) ->
+    block_equal block1 block2.
+
+    intros. 
+    (* confirm means receiving f+1 certify => at least one certify *)
+
+    (* confirm block -> lp -> 
+        early lp -> later honest nodes will not contribute to conflicting lps. 
+    *)
+    inversion H2. 
+    assert (exists com:node, is_honest_node com /\ in_committee_for com s n1 /\ let lp1:= block1.(bk_proposal) in certified_blocks com s lp1.(lp_round) = Some lp1).
+    apply commit_implies_honest_certify with (s:=s) (n:=n1). auto. auto.
+    destruct H5 as [com_node].
+    destruct H5 as [H5_1 [H5_2 H5_3]].
+
+    simpl in H5_3.
+
+    inversion H5_3.
+    apply important_lemma with (s:=s) (n:=com_node) (lp:=lp1) in H7. 2:auto. 2:auto.
+
+    destruct H7 as [H7_1 H7_2].
+
+    inversion H3.
+    assert (exists com:node, is_honest_node com /\ in_committee_for com s n2 /\ let lp:= block2.(bk_proposal) in certified_blocks com s lp.(lp_round) = Some lp).
+    apply commit_implies_honest_certify with (s:=s) (n:=n2). auto. auto.
+    destruct H5 as [com_node2].
+    destruct H5 as [H8_1 [H8_2 H8_3]].
+    simpl in H8_3.
+
+    remember (lp2.(lp_round)-lp1.(lp_round)) as r_gap.
+    induction r_gap.
+    (* in the same slot, no-one certifies a different block *)
+
+
+
+
+
+
+
+
+Admitted.
+
+Lemma safety_per_slot:
+    forall s:slot, 
+    (s = 0 \/ confirm_same_block_pred (s-1)) ->
+    forall n1 n2:node, forall block1 block2: FullBlockType,
+    is_honest_node n1 -> is_honest_node n2 ->
+    confirmed_blocks n1 s = Some block1 ->
+    confirmed_blocks n2 s = Some block2 ->
+    block_equal block1 block2.
+    intros.
+    remember (block1.(bk_proposal)) as lp1.
+    remember (block2.(bk_proposal)) as lp2.
+
+    assert ({lp1.(lp_round) <= lp2.(lp_round)} + {lp2.(lp_round)<lp1.(lp_round)}).
+    apply le_lt_dec.
+
+    destruct H4.
+    apply safety_per_slot_helper with (s:=s)(n1:=n1)(n2:=n2)(block1:=block1)(block2:=block2). auto. auto. auto. auto. auto. rewrite <- Heqlp1. rewrite <-Heqlp2. auto.
+
+
+    assert (block_equal block2 block1).
+    apply safety_per_slot_helper with (s:=s)(n1:=n2)(n2:=n1)(block1:=block2)(block2:=block1). auto. auto. auto. auto. auto. rewrite <- Heqlp2. rewrite <-Heqlp1. lia.
+    unfold block_equal. unfold block_equal in H4. auto.
+
+Qed.
+
+Lemma liveness_per_slot:
+    forall s:slot, 
+    (s = 0 \/ confirm_same_block_pred (s-1)) ->
+    forall n:node, is_honest_node n -> 
     exists block: FullBlockType,
-    state_i.(st_committed_block) = Some block) -> 
-    exists i1:nat,
-    let state_i1:= state_after_node_id n i1 in
-    state_i1.(st_slot) = S s /\
-    exists block': FullBlockType,
-    state_i1.(st_committed_block) = Some block'.
+    confirmed_blocks n s = Some block /\ confirm_slot_time n s <= enter_slot_time n s + slot_duration.
 Admitted.
-
-
-
-    
 
 
 (* safety theorem: *)
@@ -359,21 +593,32 @@ Theorem safety:
     confirmed_blocks n2 s = Some block2 ->
     block_equal block1 block2.
     intros.
-    generalize H1 H2.
-    generalize block1 block2. clear H1 H2. clear block1 block2.
-    induction s.
+    generalize H H0 H1 H2.
+    generalize n1 n2 block1 block2. clear H H0 H1 H2. clear n1 n2 block1 block2.
+    induction s. 
     intros.
-    apply safety_slot_induction_s0 with (n1:=n1) (n2:=n2) (block1:=block1) (block2:=block2). auto. auto. auto. auto. 
+    apply safety_per_slot with (s:=0)(n1:=n1)(n2:=n2)(block1:=block1)(block2:=block2). left. auto. auto. auto. auto. auto.
 
-    intro block3. intro block4. intros.
-    inversion H1. inversion H2. (*duplicate*)
+    intro n3. intro n4.
+    intro block3. intro block4.
+    intros.
+    inversion H1. (* duplicate one. show that there is a confirmed block in slot s *)
+    
     apply confirmed_block_some_implies_some in H4.
-    apply confirmed_block_some_implies_some in H5.
-    destruct H4. destruct H5.
-    assert (block_equal x x0).
-    apply IHs with (block1:=x) (block2:=x0). auto. auto.
-    (* *)
-    apply safety_slot_induction_s1 with (n1:=n1) (n2:=n2) (block1:=x) (block2:=x0) (block1':=block3) (block2':=block4) (s:=s). auto. auto. auto. auto. auto. auto. auto. auto. 
+
+    assert (confirm_same_block_pred s). 
+    unfold confirm_same_block_pred.
+    destruct H4 as [b]. exists (fullblock2aggblock b). intros.
+
+
+    inversion H3. 
+    apply one_commit_other_committed with (s:=s) (n1:=n3) (n2:=n) (block1:=b) in H6.
+    destruct H6 as [b'].
+    exists b'. split. auto.
+    apply IHs with (n1:=n)(n2:=n3) (block1:=b') (block2:=b). auto. auto. auto. auto. auto. auto. 
+
+    apply safety_per_slot with (s:=S s)(n1:=n3)(n2:=n4)(block1:=block3)(block2:=block4).
+    right. replace (S s - 1) with s by lia. auto.  auto. auto. auto. auto. 
 Qed.
 
 
@@ -381,16 +626,24 @@ Qed.
 Theorem liveness:
     forall s:slot, forall n:node, 
     is_honest_node n -> 
-        exists i:nat, let 
-            state_i:= state_after_node_id n i in
-            state_i.(st_slot) = s /\ 
-            exists block: FullBlockType, 
-            state_i.(st_committed_block) = Some block.
+        exists block: FullBlockType, 
+        confirmed_blocks n s = Some block /\ confirm_slot_time n s <= enter_slot_time n s + slot_duration.
     intros.
-    induction s.
-    apply liveness_slot_induction_s0. auto.
-    destruct IHs.
-    apply liveness_slot_induction_s1 with (i:=x). auto. auto.
+    induction s. 
+    apply liveness_per_slot with (s:=0)(n:=n). left. auto. auto. 
+
+    assert (confirm_same_block_pred s).
+    2:{apply liveness_per_slot with (s:=S s)(n:=n). right. replace (S s - 1) with s by lia. auto. auto. }
+    
+    unfold confirm_same_block_pred.
+    destruct IHs as [b]. destruct H0. exists (fullblock2aggblock b).
+    intros.
+
+    inversion H0.
+    apply one_commit_other_committed with (s:=s) (n1:=n) (n2:=n0) (block1:=b) in H4. 2:auto. 2:auto.
+    destruct H4 as [b'].
+    exists b'. split. auto.
+    apply safety with (s:=s)(n1:=n0)(n2:=n)(block1:=b')(block2:=b). auto. auto. auto. auto. 
 Qed. 
 (* ##### Part 7 ends*)
 
