note.md
@@ -4,7 +4,15 @@ On Dec 25, I restarted working on the coq proof of democratic blockchain protoco
 
 This time, I am confident that it can be finished. In order to prevent repetitive workload, I want to directly describe the complete protocol and prove the protocol. Start with the final lemmas we claim in the paper about multiple slots. 
 
-## Design choice
+Organization of this note: 
+* section1: high level design choice. 
+* section2: low-level details. 
+- 2.1 message data structures
+- 2.2 states and related data structures. 
+- 2.2 assumptions and inference
+* section3: project progress. 
+
+## 1: High-Level Design choice
 
 Previously, I worked on coq proofs of single-slot sync hotstuff protocol. New changes are the following:
 * fix the protocol change of single-slot protocol in the democratic blockchain, as formalized in the s&p submission. Note that it is different from both standard-sync hotstuff and sluggish-sync hotstuff. 
@@ -33,14 +41,9 @@ Firstly write the big results, define necessary objects. However, for these type
 Argue that the chain is infinite. Also set state_after_node_id return type to be State instead of option State. 
 
 
-## Details
-
-### outside sync hotstuff
-#### message types
-directly add an hypothesis 
-
-
-#### blockhash
+## 2: Low-Level Details
+### 2.1 Message and State - Data structures. 
+#### 2.1.1 blockhash
 
 The blockhash depends on the following fields: 
 * prevhash: defined recursively. 
@@ -50,7 +53,7 @@ The blockhash depends on the following fields:
 * vote weight (actually with its proof). 
 Note that the proof of consensus (CertProof, a list of certify messages by committee) is not included in the computation of hash. Reason: different nodes might receive different set of certify messages and proceed. If they include the set of certify messages in the computation of hash, then they the same block content might have multiple different hash values, making it hard to refer by hash values in the future. 
 
-#### State
+### 2.2 State
 States: the blockchain system is a state machine system. Every node maintains its local states, and reaches consensus on the block contents. 
 
 Committee members are determined by previous blocks, are part of the blockchain state, might be different for different nodes. Proving that they are the same for every node is a result of proving that they confirm the same block in every slot. 
@@ -61,10 +64,10 @@ keep record of the following:
 - current slot. 
 - confirmed blocks. (once confirmed, never reverted. )
   
-
+#### 2.2.1 Remark of confirmed\_blocks
 From the above framework, we can define a variable, that is the committee of each slot, in the eye of a node. 
 
-Define a full mapping: node->slot->FullBlockType? (does not assume that every block derived from teh mapping, is a valid block. )
+Define a full mapping: node->slot->FullBlockType? (does not assume that every block derived from the mapping, is a valid block. )
 
 Or use a optional mapping: node->slot->optional FullBlockType. 
 
@@ -74,23 +77,26 @@ My decision: use optional. Otherwise, I might forgot to apply the condition that
 
 
 
-#### definition of state
+#### 2.2.2 confirm a block and enter a new slot
 
 When receiving enough votes to confirm, the state does not go to the next slot immediately. Instead, it waits until receiving the aggregated proposal. This is to ensure that there exists a time, that the state confirms a block in a given slot. 
 
 
+when confirmed, stay in slot, set a timer of 1 unit, enter new slot. Using this to manually make sure that, after the event that makes the node confirm, the state remains in the current slot and committed. 
+So enter\_slot\_time = delta + previous-commit-time. 
 
-#### nodes
+#### 2.2.3 Event ordering
+Event is ordered by time. If the time is the same, also define a rule. For example, if proposal arrives at the same time as proposal-timeout, do not blame, handle proposal arrival first. 
+
+### 2.3 Blockchain Assumptions
+#### 2.3.1 bound on number of nodes
 
 note that, the set of nodes must be bounded. Otherwise, a node might receive infinite incoming messages in one slot, thus not able to prove liveness. Will add a hypothesis, saying that each node at most receives a bounded amount of messsages from boundedly many nodes in every slot. Thus can show liveness with concrete time bounds. 
 
 
 
-#### new slot
 
-when confirmed, stay in slot, set a timer of 1 unit, enter new slot. Using this to manually make sure that, after the event that makes the node confirm, the state remains in the current slot and committed. 
-
-## work record
+## 3: work record
 There are two ultimate goals: proving safety and proving liveness. If I only consider proving safety first, I might end up with writing a lot of code, but missing the necessary details for proving livess. 
 
 
@@ -105,7 +111,22 @@ Stating that other honest nodes also commit the same block, is the safety theore
 
 Therefore, must develop the state transition and triggers now. BUT don't forget backward engineering. How does the safety lemma breaks apart? 
 
-## coq notes
+#### Break safety:
+- safety\_per\_slot: if every honest node confirms the same block in the previous slot, then if any two honest nodes confirm blocks in the current slot, they must confirm the same block. 
+- one\_commit\_other\_committed: this is a lemma that can be easily proved, when the message forwarding is described. Others might not commit the same block. 
+- Hypothesis: none-keeps-none -> implies some-prev-is-some. Part of the state machine definition, must confirm a block before proceeding to confirm the next slot. 
+
+#### Break liveness:
+- liveness\_per\_slot: condition is, every honest node confirms the same block in the previous slot. 
+- one\_commit\_other\_committed: to show that in the previous slot, everyone committed. 
+- safety: since everyone committed in the previous slot, they committed the same block in previous slot. 
+
+Therefore, in the next stage, I should prove the following lemmas:
+* safety per slot: 
+* liveness per slot:
+* one commit other committed: this is much more detailed results. 
+
+## 4: coq notes
 
 How to use a lemma that states exists something.  How to make it explicit. 
 
@@ -114,10 +135,3 @@ example: exists e, var = some e.
 How to replace var with some e. 
 
 directly use destruct. 
-
-
-
-
-
-## Bug?
-
